@prefix coreo: <http://purl.org/coreo#> .
@prefix dcat: <http://www.w3.org/ns/dcat#> .
@prefix dct: <http://purl.org/dc/terms/> .
@prefix foaf: <http://xmlns.com/foaf/0.1/> .
@prefix gufo: <http://purl.org/nemo/gufo#> .
@prefix owl: <http://www.w3.org/2002/07/owl#> .
@prefix rdf: <http://www.w3.org/1999/02/22-rdf-syntax-ns#> .
@prefix rdfs: <http://www.w3.org/2000/01/rdf-schema#> .
@prefix vann: <http://purl.org/vocab/vann/> .
@prefix voaf: <http://purl.org/vocommons/voaf#> .
@prefix xml: <http://www.w3.org/XML/1998/namespace> .
@prefix xsd: <http://www.w3.org/2001/XMLSchema#> .
@base <http://purl.org/coreo> .

<http://purl.org/coreo> rdf:type owl:Ontology ;
                         dcat:landingPage <http://purl.org/coreo/git> ;
                         dct:bibliographicCitation "R. F. Calhau, J. P. A. Almeida, T. P. Sales, G. Guizzardi, \\\"Core-O: A Competence Reference Ontology\\\", 2023, http://purl.org/coreo"@en ;
                         dct:contributor <https://orcid.org/0000-0003-2736-7817>;
                         dct:created "2023-05-08"^^xsd:date ;
                         dct:creator <https://orcid.org/0009-0006-6051-2165>, <https://orcid.org/0000-0002-9819-3781>, <https://orcid.org/0000-0002-5385-5761>, <https://orcid.org/0000-0002-3452-553X>;
                         dct:description "An ontology to describe competences and human capabilities"@en ;
                         dct:identifier "http://purl.org/coreo/"^^xsd:anyURI ;
                         dct:issued "2023-05-08"^^xsd:date ;
                         dct:language <http://id.loc.gov/vocabulary/iso639-1/en> ;                         
                         dct:license "https://creativecommons.org/licenses/by/4.0/legalcode"^^xsd:anyURI ;
                         dct:modified "2024-02-01" ;
                         dct:publisher <https://www.utwente.nl/eemcs/scs/>, <https://nemo.inf.ufes.br/> ;
                         dct:title "Core-o: Competence Reference Ontology"@en ;
                         foaf:homepage <http://purl.org/coreo/doc> ;
                         owl:priorVersion <http://purl.org/coreo/v1.0.0> ;
                         owl:versionInfo "1.0.1"@en ;
                         owl:versionIRI <http://purl.org/coreo/1.0.1> ;
                         vann:preferredNamespacePrefix "coreo";
                         vann:preferredNamespaceUri "http://purl.org/coreo#"^^xsd:anyURI ;
                         rdfs:comment """Core-O is a well-founded competence reference ontology that accounts for competence-related elements such as knowledge, attitudes, and skills; also countenance their performance---related to tasks, their context, and outcomes---as well as their evolution over time (proficiency). This ontology is based on the Unified Foundational Ontology (Guizzardi, 2005), more specifically using gUFO (gentle UFO), a UFO-based lightweight ontology.
The ontology was based on these works: (CALHAU et al., 2021) and (CALHAU et al., 2023)

It was created to support: (i) semantically annotate competence-related artifacts such as curriculum, job vacancy, learning objects, resources, professional profiles, task logs, logbooks, and learning diaries; (ii) semantically inter-operate and integrate professional data concerning internal system (from organizations, VET institutions) and external ones (e.g., professional networks as LinkedIn); (iii) support the semantic search to find the best professional to an occupation, or to find the best occupation to a professional; (iv) support the skill/competence matching in gap analysis; (v) support competence/skill identification/assessment based on ontology-driven data and text mining in competence-related artifacts, such as learning diary, logbook, or task logs from control version tools as Github.


For background information on the reference ontology, see: 

1. CALHAU, Rodrigo F.; AZEVEDO, Carlos LB; ALMEIDA, João Paulo A. Towards Ontology-based Competence Modeling in Enterprise Architecture. In: 2021 IEEE 25th International Enterprise Distributed Object Computing Conference (EDOC). IEEE, 2021. p. 71-81.
2. CALHAU, Rodrigo F.; ALMEIDA, João Paulo A. Zooming in on Competences in Ontology-Based Enterprise Architecture Modeling. In: Enterprise Design, Operations, and Computing. EDOC 2022 Workshops: IDAMS, SoEA4EE, TEAR, EDOC Forum, Demonstrations Track and Doctoral Consortium, Bozen-Bolzano, Italy, October 4–7, 2022, Revised Selected Papers. Cham: Springer International Publishing, 2023. p. 198-213.
3. GUIZZARDI, Giancarlo. Ontological foundations for structural conceptual models. 2005.

Cite this work as: 
R. F. Calhau, J. P. A. Almeida, T. P. Sales, G. Guizzardi, \\\"Core-O: A Competence Reference Ontology\\\", 2023, http://purl.org/coreo

This work is distributed under Creative Commons Attribution License CC BY 4.0 <https://creativecommons.org/licenses/by/4.0/legalcode>.


For the source repository, see: <http://purl.org/coreo/git>"""@en .



#################################################################
#    Object Properties
#################################################################

###  http://purl.org/coreo#bringsAbout
coreo:bringsAbout rdf:type owl:ObjectProperty ;
                  rdfs:domain coreo:TaskType ;
                  rdfs:range gufo:SituationType ;
                  rdfs:comment "Details the SituationType that a coreo:TaskType can result"@en ;
                  rdfs:label "bringsAbout"@en .


###  http://purl.org/coreo#broughtAboutHumanTask
coreo:broughtAboutHumanTask rdf:type owl:ObjectProperty ;
                            rdfs:subPropertyOf gufo:broughtAbout ;
                            rdfs:domain coreo:CompetenceOutcome ;
                            rdfs:range coreo:HumanTask ;
                            rdfs:label ""@en .


###  http://purl.org/coreo#capabilityRequiringRoleHasField
coreo:capabilityRequiringRoleHasField rdf:type owl:ObjectProperty ;
                                      rdfs:domain coreo:CapabilityRequiringRole ;
                                      rdfs:range coreo:Field ;
                                      rdfs:comment "Describes the field of a coreo:CapabilityRequiringRole"@en ;
                                      rdfs:label "hasField"@en .


###  http://purl.org/coreo#characterizedBy
coreo:characterizedBy rdf:type owl:ObjectProperty ;
                      rdfs:subPropertyOf coreo:describedBy ;
                      rdfs:domain coreo:ArtifactType ;
                      rdfs:range coreo:MomentType ;
                      rdfs:comment "Relationship used to detail a coreo:ArtifactType"@en ;
                      rdfs:label "characterizedBy"@en .


###  http://purl.org/coreo#competenceContextContributedToTriggerHumanTask
coreo:competenceContextContributedToTriggerHumanTask rdf:type owl:ObjectProperty ;
                                                     rdfs:subPropertyOf gufo:contributedToTrigger ;
                                                     rdfs:domain coreo:CompetenceContext ;
                                                     rdfs:range coreo:HumanTask ;
                                                     rdfs:comment "Identifies a coreo:HumanTask that the coreo:CompetenceContext contributed to trigger."@en ;
                                                     rdfs:label "activatesTask"@en .


###  http://purl.org/coreo#concerns
coreo:concerns rdf:type owl:ObjectProperty ;
               rdfs:subPropertyOf coreo:describedBy ;
               rdfs:domain coreo:TaskType ;
               rdfs:range coreo:ArtifactType ;
               rdfs:comment "Relationship used to detail a coreo:TaskType"@en ;
               rdfs:label "concernsArtifact"@en .


###  http://purl.org/coreo#concerns_1
coreo:concerns_1 rdf:type owl:ObjectProperty ;
                 rdfs:subPropertyOf coreo:describedBy ;
                 rdfs:domain coreo:TaskType ;
                 rdfs:range coreo:ResourceType ;
                 rdfs:comment "Relationship used to detail a coreo:TaskType"@en ;
                 rdfs:label "concernsResource"@en .


###  http://purl.org/coreo#constitutes
coreo:constitutes rdf:type owl:ObjectProperty ;
                  rdfs:subPropertyOf coreo:constitutesType ;
                  rdfs:domain coreo:HumanAspectType ;
                  rdfs:range coreo:HumanAspectType ;
                  rdfs:comment "Describes the constitutive relationship between coreo:HumanAspectTypes manifested as parthood relationships between their instances"@en ;
                  rdfs:label "constitutesAspect"@en .


###  http://purl.org/coreo#constitutesType
coreo:constitutesType rdf:type owl:ObjectProperty ;
                      rdfs:domain gufo:Type ;
                      rdfs:range gufo:Type ;
                      rdfs:comment "Describes the constitutive relationship between types manifested as parthood relationships between their instances"@en ;
                      rdfs:label "constitutesType"@en .


###  http://purl.org/coreo#contributesTo
coreo:contributesTo rdf:type owl:ObjectProperty ;
                    rdfs:domain coreo:HumanQuality ;
                    rdfs:range coreo:PersonalCompetence ;
                    rdfs:comment "Describes the contribution relation between a coreo:HumanQuality and a coreo:PersonalCompetence"@en ;
                    rdfs:label "contributesTo"@en .


###  http://purl.org/coreo#definedInTermsOf
coreo:definedInTermsOf rdf:type owl:ObjectProperty ;
                       rdfs:subPropertyOf coreo:describedBy ;
                       rdfs:domain coreo:HumanCapabilityType ;
                       rdfs:range coreo:TaskType ;
                       rdfs:comment "Relationship used to detail a coreo:HumanCapabilityType"@en ;
                       rdfs:label "definedInTermsOf"@en .


###  http://purl.org/coreo#dependsOn
coreo:dependsOn rdf:type owl:ObjectProperty ;
                rdfs:subPropertyOf coreo:dependsOnType ;
                rdfs:domain coreo:TaskType ;
                rdfs:range coreo:TaskType ;
                rdfs:comment "Describes the dependence relationship between types manifested as dependence relationships between their instances"@en ;
                rdfs:label "dependsOnTask"@en .


###  http://purl.org/coreo#dependsOnType
coreo:dependsOnType rdf:type owl:ObjectProperty ;
                    rdfs:domain gufo:Type ;
                    rdfs:range gufo:Type ;
                    rdfs:comment "Describes the dependence relationship between types manifested as dependence relationships between their instances"@en ;
                    rdfs:label "dependsOnType"@en .


###  http://purl.org/coreo#dependsOn_1
coreo:dependsOn_1 rdf:type owl:ObjectProperty ;
                  rdfs:subPropertyOf coreo:dependsOnType ;
                  rdfs:domain coreo:ArtifactType ;
                  rdfs:range coreo:ArtifactType ;
                  rdfs:comment "Describes the dependence relationship between types manifested as dependence relationships between their instances"@en ;
                  rdfs:label "dependsOnArtifact"@en .


###  http://purl.org/coreo#dependsOn_2
coreo:dependsOn_2 rdf:type owl:ObjectProperty ;
                  rdfs:subPropertyOf coreo:dependsOnType ;
                  rdfs:domain coreo:HumanAspectType ;
                  rdfs:range coreo:HumanAspectType ;
                  rdfs:comment "Describes the dependence relationship between types manifested as dependence relationships between their instances"@en ;
                  rdfs:label "dependsOnHumanAspect"@en .


###  http://purl.org/coreo#dependsOn_3
coreo:dependsOn_3 rdf:type owl:ObjectProperty ;
                  rdfs:subPropertyOf coreo:dependsOnType ;
                  rdfs:domain coreo:CapabilityRequiringRole ;
                  rdfs:range coreo:CapabilityRequiringRole ;
                  rdfs:comment "Describes the dependence relationship between types manifested as dependence relationships between their instances"@en ;
                  rdfs:label "dependsOnRole"@en .


###  http://purl.org/coreo#describedBy
coreo:describedBy rdf:type owl:ObjectProperty ;
                  rdfs:domain gufo:Type ;
                  rdfs:range gufo:Type ;
                  rdfs:comment "Relationship used to detail a type"@en ;
                  rdfs:label "describedBy"@en .


###  http://purl.org/coreo#enables
coreo:enables rdf:type owl:ObjectProperty ;
              rdfs:domain coreo:HumanCapabilityType ;
              rdfs:range gufo:SituationType ;
              rdfs:comment "Relationship used to detail types of contexts that activates HumanCapabilityTypes"@en ;
              rdfs:label "enablesSituationType"@en .


###  http://purl.org/coreo#evidencedBy
coreo:evidencedBy rdf:type owl:ObjectProperty ;
                  rdfs:domain coreo:HumanAspect ;
                  rdfs:range coreo:Evidence ;
                  rdfs:comment "evidances of a coreo:HumanAspect"@en ;
                  rdfs:label "evidencedBy"@en .


###  http://purl.org/coreo#inheresIn
coreo:inheresIn rdf:type owl:ObjectProperty ;
                rdfs:subPropertyOf gufo:inheresIn ;
                rdf:type owl:FunctionalProperty ,
                         owl:AsymmetricProperty ,
                         owl:IrreflexiveProperty ;
                rdfs:domain coreo:Proficiency ;
                rdfs:range coreo:HumanCapability ;
                rdfs:comment "relates a coreo:Proficiency to the correspondent coreo:HumanCapability"@en ;
                rdfs:label "inheresInHumanCapability"@en .


###  http://purl.org/coreo#inheresIn_1
coreo:inheresIn_1 rdf:type owl:ObjectProperty ;
                  rdfs:subPropertyOf coreo:inheresIn_2 ;
                  rdf:type owl:FunctionalProperty ,
                           owl:AsymmetricProperty ,
                           owl:IrreflexiveProperty ;
                  rdfs:domain coreo:HumanCapability ;
                  rdfs:range coreo:Person ;
                  rdfs:comment "relates the coreo:HumanCapability to the correspondent coreo:Person"@en ;
                  rdfs:label "CapabilityInheresInPerson"@en .


###  http://purl.org/coreo#inheresIn_2
coreo:inheresIn_2 rdf:type owl:ObjectProperty ;
                  rdfs:subPropertyOf gufo:inheresIn ;
                  rdf:type owl:FunctionalProperty ,
                           owl:AsymmetricProperty ,
                           owl:IrreflexiveProperty ;
                  rdfs:domain coreo:HumanAspect ;
                  rdfs:range coreo:Person ;
                  rdfs:comment "relates the coreo:HumanAspect to the correspondent coreo:Person"@en ;
                  rdfs:label "inheresInPerson"@en .


###  http://purl.org/coreo#isDefinedBy
coreo:isDefinedBy rdf:type owl:ObjectProperty ;
                  rdfs:subPropertyOf coreo:describedBy ;
                  rdfs:domain coreo:CapabilityRequiringRole ;
                  rdfs:range coreo:HumanCapabilityType ;
                  rdfs:comment "Relationship used to detail a coreo:HumanCapabilityType"@en ;
                  rdfs:label "isDefinedBy"@en .


###  http://purl.org/coreo#performed
coreo:performed rdf:type owl:ObjectProperty ;
                rdfs:subPropertyOf gufo:participatedIn ;
                rdfs:domain coreo:Person ;
                rdfs:range coreo:HumanTask ;
                rdfs:comment "participation of a person in a human task"@en ;
                rdfs:label "performed"@en .


###  http://purl.org/coreo#personalCompetenceHasAttitude
coreo:personalCompetenceHasAttitude rdf:type owl:ObjectProperty ;
                                    rdfs:subPropertyOf gufo:isAspectProperPartOf ;
                                    rdfs:domain coreo:PersonalCompetence ;
                                    rdfs:range coreo:Attitude ;
                                    rdfs:comment "parthood relation between a competence and attitude"@en ;
                                    rdfs:label "hasAttitude"@en .


###  http://purl.org/coreo#personalCompetenceHasHumanAspect
coreo:personalCompetenceHasHumanAspect rdf:type owl:ObjectProperty ;
                                       rdfs:subPropertyOf gufo:isAspectProperPartOf ;
                                       rdfs:domain coreo:PersonalCompetence ;
                                       rdfs:range coreo:HumanAspect ;
                                       rdfs:comment "parthood relation between a competence and human aspect"@en ;
                                       rdfs:label "hasHumanAspect"@en .


###  http://purl.org/coreo#personalCompetenceHasKnowledge
coreo:personalCompetenceHasKnowledge rdf:type owl:ObjectProperty ;
                                     rdfs:subPropertyOf gufo:isAspectProperPartOf ;
                                     rdfs:domain coreo:PersonalCompetence ;
                                     rdfs:range coreo:Knowledge ;
                                     rdfs:comment "parthood relation between a competence and knowledge"@en ;
                                     rdfs:label "hasKnowledge"@en .


###  http://purl.org/coreo#personalCompetenceHasPersonalCompetence
coreo:personalCompetenceHasPersonalCompetence rdf:type owl:ObjectProperty ;
                                              rdfs:subPropertyOf gufo:isAspectProperPartOf ;
                                              rdfs:domain coreo:PersonalCompetence ;
                                              rdfs:range coreo:PersonalCompetence ;
                                              rdfs:comment "parthood relation between a competence and other competence"@en ;
                                              rdfs:label "hasCompetence"@en .


###  http://purl.org/coreo#personalCompetenceHasSkill
coreo:personalCompetenceHasSkill rdf:type owl:ObjectProperty ;
                                 rdfs:subPropertyOf gufo:isAspectProperPartOf ;
                                 rdfs:domain coreo:PersonalCompetence ;
                                 rdfs:range coreo:Skill ;
                                 rdfs:comment "parthood relation between a competence and skill"@en ;
                                 rdfs:label "hasSkill"@en .


###  http://purl.org/coreo#specializes
coreo:specializes rdf:type owl:ObjectProperty ;
                  rdfs:subPropertyOf coreo:specializes_1 ;
                  rdfs:domain coreo:ArtifactType ;
                  rdfs:range coreo:ArtifactType ;
                  rdfs:comment "specialization relation between types symbolizing the types that are instances of other type"@en ;
                  rdfs:label "specializesArtifact"@en .


###  http://purl.org/coreo#specializes_1
coreo:specializes_1 rdf:type owl:ObjectProperty ;
                    rdfs:domain gufo:Type ;
                    rdfs:range gufo:Type ;
                    rdfs:comment "specialization relation between types symbolizing the types that are instances of other type"@en ;
                    rdfs:label "specializes"@en .


###  http://purl.org/coreo#specializes_2
coreo:specializes_2 rdf:type owl:ObjectProperty ;
                    rdfs:subPropertyOf coreo:specializes_1 ;
                    rdfs:domain coreo:HumanAspectType ;
                    rdfs:range coreo:HumanAspectType ;
                    rdfs:comment "specialization relation between types symbolizing the types that are instances of other type"@en ;
                    rdfs:label "specializesAspect"@en .


###  http://purl.org/coreo#specializes_3
coreo:specializes_3 rdf:type owl:ObjectProperty ;
                    rdfs:subPropertyOf coreo:specializes_1 ;
                    rdfs:domain coreo:TaskType ;
                    rdfs:range coreo:TaskType ;
                    rdfs:comment "specialization relation between types symbolizing the types that are instances of other type"@en ;
                    rdfs:label "specializesTask"@en .


###  http://purl.org/coreo#specializes_4
coreo:specializes_4 rdf:type owl:ObjectProperty ;
                    rdfs:subPropertyOf coreo:specializes_1 ;
                    rdfs:domain coreo:CapabilityRequiringRole ;
                    rdfs:range coreo:CapabilityRequiringRole ;
                    rdfs:comment "specialization relation between types symbolizing the types that are instances of other type"@en ;
                    rdfs:label "specializesRole"@en .


###  http://purl.org/coreo#standsIn
coreo:standsIn rdf:type owl:ObjectProperty ;
               rdfs:subPropertyOf gufo:standsIn ;
               rdfs:domain coreo:Resource ;
               rdfs:range coreo:CompetenceContext ;
               rdfs:comment "Details the coreo:Resource that stands in a coreo:CompetenceContext"@en ;
               rdfs:label "standsInContext"@en .


###  http://purl.org/coreo#standsIn_1
coreo:standsIn_1 rdf:type owl:ObjectProperty ;
                 rdfs:subPropertyOf gufo:standsIn ;
                 rdfs:domain coreo:Artifact ;
                 rdfs:range coreo:CompetenceContext ;
                 rdfs:comment "Details the coreo:Artifact that stands in a coreo:CompetenceContext"@en ;
                 rdfs:label "standsInContext"@en .


###  http://purl.org/coreo#standsIn_2
coreo:standsIn_2 rdf:type owl:ObjectProperty ;
                 rdfs:subPropertyOf gufo:standsIn ;
                 rdfs:domain coreo:Artifact ;
                 rdfs:range coreo:CompetenceOutcome ;
                 rdfs:comment "Details the coreo:Artifact that stands in a coreo:CompetenceOutcome"@en ;
                 rdfs:label "standsInOutcome"@en .


###  http://purl.org/coreo#wasGeneratedIn
coreo:wasGeneratedIn rdf:type owl:ObjectProperty ;
                     rdfs:subPropertyOf gufo:wasCreatedIn ;
                     rdfs:domain coreo:TaskOutput ;
                     rdfs:range coreo:HumanTask ;
                     rdfs:comment "output generation from a coreo:HumanTask"@en ;
                     rdfs:label "wasGeneratedIn"@en .


###  http://purl.org/coreo#wasManifestedIn
coreo:wasManifestedIn rdf:type owl:ObjectProperty ;
                      rdfs:subPropertyOf gufo:manifestedIn ;
                      rdfs:domain coreo:HumanAspect ;
                      rdfs:range coreo:HumanTask ;
                      rdfs:comment "Identifies a coreo:HumanTask in which the coreo:HumanAspect is manifested."@en ;
                      rdfs:label "wasManifestedInTask"@en .


###  http://purl.org/coreo#wasManifestedIn_1
coreo:wasManifestedIn_1 rdf:type owl:ObjectProperty ;
                        rdfs:subPropertyOf gufo:manifestedIn ;
                        rdfs:domain coreo:HumanCapability ;
                        rdfs:range coreo:HumanTask ;
                        rdfs:comment "Identifies a coreo:HumanTask in which the coreo:HumanCapability is manifested."@en ;
                        rdfs:label "wasManifestedIn"@en .


###  http://purl.org/coreo#wasUsedIn
coreo:wasUsedIn rdf:type owl:ObjectProperty ;
                rdfs:subPropertyOf gufo:participatedIn ;
                rdfs:domain coreo:TaskInput ;
                rdfs:range coreo:HumanTask ;
                rdfs:comment "usage of a artifact in a human task as input"@en ;
                rdfs:label "wasUsedIn"@en .


###  http://purl.org/coreo#wasUsedIn_1
coreo:wasUsedIn_1 rdf:type owl:ObjectProperty ;
                  rdfs:subPropertyOf gufo:participatedIn ;
                  rdfs:domain coreo:Resource ;
                  rdfs:range coreo:HumanTask ;
                  rdfs:comment "usage of an object in a human task as a resource"@en ;
                  rdfs:label "wasUsedIn"@en .


#################################################################
#    Classes
#################################################################

###  http://purl.org/coreo#Agent
coreo:Agent rdf:type owl:Class ;
            rdfs:subClassOf gufo:Object .


###  http://purl.org/coreo#Artifact
coreo:Artifact rdf:type owl:Class ;
               rdfs:subClassOf gufo:Object .


###  http://purl.org/coreo#ArtifactType
coreo:ArtifactType rdf:type owl:Class ;
                   rdfs:subClassOf coreo:SubstantialType .


###  http://purl.org/coreo#Attitude
coreo:Attitude rdf:type owl:Class ;
               rdfs:subClassOf coreo:HumanAspect .


###  http://purl.org/coreo#AttitudeType
coreo:AttitudeType rdf:type owl:Class ;
                   rdfs:subClassOf coreo:HumanAspectType .


###  http://purl.org/coreo#CapabilityRequiringRole
coreo:CapabilityRequiringRole rdf:type owl:Class ;
                              rdfs:subClassOf gufo:Role .


###  http://purl.org/coreo#CompetenceContext
coreo:CompetenceContext rdf:type owl:Class ;
                        rdfs:subClassOf gufo:Situation ,
                                        [ rdf:type owl:Restriction ;
                                          owl:onProperty coreo:competenceContextContributedToTriggerHumanTask ;
                                          owl:someValuesFrom coreo:HumanTask
                                        ] .


###  http://purl.org/coreo#CompetenceOutcome
coreo:CompetenceOutcome rdf:type owl:Class ;
                        rdfs:subClassOf gufo:Situation .


###  http://purl.org/coreo#Evidence
coreo:Evidence rdf:type owl:Class ;
               rdfs:subClassOf gufo:ConcreteIndividual .


###  http://purl.org/coreo#Field
coreo:Field rdf:type owl:Class ;
            rdfs:subClassOf gufo:ConcreteIndividualType .


###  http://purl.org/coreo#HumanAspect
coreo:HumanAspect rdf:type owl:Class ;
                  rdfs:subClassOf gufo:IntrinsicMode ,
                                  [ rdf:type owl:Restriction ;
                                    owl:onProperty coreo:inheresIn_2 ;
                                    owl:qualifiedCardinality "1"^^xsd:nonNegativeInteger ;
                                    owl:onClass coreo:Person
                                  ] .


###  http://purl.org/coreo#HumanAspectPhase
coreo:HumanAspectPhase rdf:type owl:Class ;
                       rdfs:subClassOf coreo:HumanAspectType ,
                                       gufo:Phase .


###  http://purl.org/coreo#HumanAspectType
coreo:HumanAspectType rdf:type owl:Class ;
                      rdfs:subClassOf coreo:MomentType .


###  http://purl.org/coreo#HumanCapability
coreo:HumanCapability rdf:type owl:Class ;
                      owl:equivalentClass [ rdf:type owl:Class ;
                                            owl:unionOf ( coreo:PersonalCompetence
                                                          coreo:Skill
                                                        )
                                          ] ;
                      rdfs:subClassOf coreo:HumanAspect ,
                                      [ rdf:type owl:Restriction ;
                                        owl:onProperty coreo:wasManifestedIn_1 ;
                                        owl:someValuesFrom coreo:HumanTask
                                      ] ,
                                      [ rdf:type owl:Restriction ;
                                        owl:onProperty [ owl:inverseOf coreo:inheresIn
                                                       ] ;
                                        owl:someValuesFrom coreo:Proficiency
                                      ] ,
                                      [ rdf:type owl:Restriction ;
                                        owl:onProperty coreo:inheresIn_1 ;
                                        owl:qualifiedCardinality "1"^^xsd:nonNegativeInteger ;
                                        owl:onClass coreo:Person
                                      ] .


###  http://purl.org/coreo#HumanCapabilityType
coreo:HumanCapabilityType rdf:type owl:Class ;
                          rdfs:subClassOf coreo:HumanAspectType .


###  http://purl.org/coreo#HumanQuality
coreo:HumanQuality rdf:type owl:Class ;
                   rdfs:subClassOf coreo:HumanAspect .


###  http://purl.org/coreo#HumanTask
coreo:HumanTask rdf:type owl:Class ;
                rdfs:subClassOf gufo:Event ,
                                [ rdf:type owl:Restriction ;
                                  owl:onProperty [ owl:inverseOf coreo:performed
                                                 ] ;
                                  owl:someValuesFrom coreo:Person
                                ] ,
                                [ rdf:type owl:Restriction ;
                                  owl:onProperty [ owl:inverseOf coreo:wasGeneratedIn
                                                 ] ;
                                  owl:someValuesFrom coreo:TaskOutput
                                ] ,
                                [ rdf:type owl:Restriction ;
                                  owl:onProperty [ owl:inverseOf coreo:wasManifestedIn
                                                 ] ;
                                  owl:someValuesFrom coreo:HumanAspect
                                ] ,
                                [ rdf:type owl:Restriction ;
                                  owl:onProperty [ owl:inverseOf coreo:wasUsedIn
                                                 ] ;
                                  owl:someValuesFrom coreo:TaskInput
                                ] ,
                                [ rdf:type owl:Restriction ;
                                  owl:onProperty [ owl:inverseOf coreo:wasUsedIn_1
                                                 ] ;
                                  owl:someValuesFrom coreo:Resource
                                ] ,
                                [ rdf:type owl:Restriction ;
                                  owl:onProperty [ owl:inverseOf coreo:competenceContextContributedToTriggerHumanTask
                                                 ] ;
                                  owl:minQualifiedCardinality "1"^^xsd:nonNegativeInteger ;
                                  owl:onClass coreo:CompetenceContext
                                ] .


###  http://purl.org/coreo#HumanTrait
coreo:HumanTrait rdf:type owl:Class ;
                 rdfs:subClassOf coreo:HumanAspect .


###  http://purl.org/coreo#Knowledge
coreo:Knowledge rdf:type owl:Class ;
                rdfs:subClassOf coreo:HumanAspect .


###  http://purl.org/coreo#KnowledgeType
coreo:KnowledgeType rdf:type owl:Class ;
                    rdfs:subClassOf coreo:HumanAspectType .


###  http://purl.org/coreo#MomentType
coreo:MomentType rdf:type owl:Class ;
                 rdfs:subClassOf gufo:EndurantType .


###  http://purl.org/coreo#Object
coreo:Object rdf:type owl:Class ;
             rdfs:subClassOf gufo:FunctionalComplex .


###  http://purl.org/coreo#Person
coreo:Person rdf:type owl:Class ;
             rdfs:subClassOf coreo:Agent ,
                             [ rdf:type owl:Restriction ;
                               owl:onProperty [ owl:inverseOf coreo:inheresIn_1
                                              ] ;
                               owl:qualifiedCardinality "1"^^xsd:nonNegativeInteger ;
                               owl:onClass coreo:HumanCapability
                             ] .


###  http://purl.org/coreo#PersonalCompetence
coreo:PersonalCompetence rdf:type owl:Class ;
                         rdfs:subClassOf coreo:HumanCapability ;
                         owl:disjointWith coreo:Skill .


###  http://purl.org/coreo#PersonalCompetenceType
coreo:PersonalCompetenceType rdf:type owl:Class ;
                             rdfs:subClassOf coreo:HumanCapabilityType .


###  http://purl.org/coreo#Proficiency
coreo:Proficiency rdf:type owl:Class ;
                  rdfs:subClassOf gufo:Quality ,
                                  [ rdf:type owl:Restriction ;
                                    owl:onProperty coreo:inheresIn ;
                                    owl:qualifiedCardinality "1"^^xsd:nonNegativeInteger ;
                                    owl:onClass coreo:HumanCapability
                                  ] .


###  http://purl.org/coreo#Resource
coreo:Resource rdf:type owl:Class ;
               rdfs:subClassOf gufo:Object .


###  http://purl.org/coreo#ResourceType
coreo:ResourceType rdf:type owl:Class ;
                   rdfs:subClassOf coreo:SubstantialType .


###  http://purl.org/coreo#Skill
coreo:Skill rdf:type owl:Class ;
            rdfs:subClassOf coreo:HumanCapability .


###  http://purl.org/coreo#SkillType
coreo:SkillType rdf:type owl:Class ;
                rdfs:subClassOf coreo:HumanCapabilityType .


###  http://purl.org/coreo#SubstantialType
coreo:SubstantialType rdf:type owl:Class ;
                      rdfs:subClassOf gufo:EndurantType .


###  http://purl.org/coreo#TaskInput
coreo:TaskInput rdf:type owl:Class ;
                rdfs:subClassOf coreo:Artifact .


###  http://purl.org/coreo#TaskOutput
coreo:TaskOutput rdf:type owl:Class ;
                 rdfs:subClassOf coreo:Artifact .


###  http://purl.org/coreo#TaskType
coreo:TaskType rdf:type owl:Class ;
               rdfs:subClassOf gufo:EventType .


#################################################################
#    Individuals
#################################################################

###  http://purl.org/coreo
<http://purl.org/coreo> rdf:type owl:NamedIndividual ,
                                 voaf:Vocabulary .


###  http://purl.org/coreo#Agent
coreo:Agent rdf:type owl:NamedIndividual ,
                     gufo:Category .


###  http://purl.org/coreo#Artifact
coreo:Artifact rdf:type owl:NamedIndividual ,
                        gufo:Category .


###  http://purl.org/coreo#ArtifactType
coreo:ArtifactType rdf:type owl:NamedIndividual .


###  http://purl.org/coreo#Attitude
coreo:Attitude rdf:type owl:NamedIndividual ,
                        gufo:Kind .


###  http://purl.org/coreo#AttitudeType
coreo:AttitudeType rdf:type owl:NamedIndividual .


###  http://purl.org/coreo#CapabilityRequiringRole
coreo:CapabilityRequiringRole rdf:type owl:NamedIndividual .


###  http://purl.org/coreo#CompetenceContext
coreo:CompetenceContext rdf:type owl:NamedIndividual ,
                                 gufo:SituationType .


###  http://purl.org/coreo#CompetenceOutcome
coreo:CompetenceOutcome rdf:type owl:NamedIndividual ,
                                 gufo:SituationType .


###  http://purl.org/coreo#EndurantType
coreo:EndurantType rdf:type owl:NamedIndividual .


###  http://purl.org/coreo#Evidence
coreo:Evidence rdf:type owl:NamedIndividual ,
                        gufo:Category .


###  http://purl.org/coreo#Field
coreo:Field rdf:type owl:NamedIndividual .


###  http://purl.org/coreo#HumanAspect
coreo:HumanAspect rdf:type owl:NamedIndividual ,
                           gufo:Category .


###  http://purl.org/coreo#HumanAspectPhase
coreo:HumanAspectPhase rdf:type owl:NamedIndividual .


###  http://purl.org/coreo#HumanAspectType
coreo:HumanAspectType rdf:type owl:NamedIndividual .


###  http://purl.org/coreo#HumanCapability
coreo:HumanCapability rdf:type owl:NamedIndividual ,
                               gufo:Kind .


###  http://purl.org/coreo#HumanCapabilityType
coreo:HumanCapabilityType rdf:type owl:NamedIndividual .


###  http://purl.org/coreo#HumanQuality
coreo:HumanQuality rdf:type owl:NamedIndividual ,
                            gufo:Category .


###  http://purl.org/coreo#HumanTask
coreo:HumanTask rdf:type owl:NamedIndividual ,
                         gufo:EventType .


###  http://purl.org/coreo#HumanTrait
coreo:HumanTrait rdf:type owl:NamedIndividual ,
                          gufo:Category .


###  http://purl.org/coreo#Knowledge
coreo:Knowledge rdf:type owl:NamedIndividual ,
                         gufo:Kind .


###  http://purl.org/coreo#KnowledgeType
coreo:KnowledgeType rdf:type owl:NamedIndividual .


###  http://purl.org/coreo#MomentType
coreo:MomentType rdf:type owl:NamedIndividual .


###  http://purl.org/coreo#Object
coreo:Object rdf:type owl:NamedIndividual ,
                      gufo:Category .


###  http://purl.org/coreo#PerdurantType
coreo:PerdurantType rdf:type owl:NamedIndividual .


###  http://purl.org/coreo#Person
coreo:Person rdf:type owl:NamedIndividual ,
                      gufo:Kind .


###  http://purl.org/coreo#PersonalCompetence
coreo:PersonalCompetence rdf:type owl:NamedIndividual ,
                                  gufo:SubKind .


###  http://purl.org/coreo#PersonalCompetenceType
coreo:PersonalCompetenceType rdf:type owl:NamedIndividual .


###  http://purl.org/coreo#Phase
coreo:Phase rdf:type owl:NamedIndividual .


###  http://purl.org/coreo#PhysicalAgent
coreo:PhysicalAgent rdf:type owl:NamedIndividual ,
                             gufo:Category .


###  http://purl.org/coreo#Proficiency
coreo:Proficiency rdf:type owl:NamedIndividual ,
                           gufo:Kind .


###  http://purl.org/coreo#Resource
coreo:Resource rdf:type owl:NamedIndividual ,
                        gufo:RoleMixin .


###  http://purl.org/coreo#ResourceType
coreo:ResourceType rdf:type owl:NamedIndividual .


###  http://purl.org/coreo#Role
coreo:Role rdf:type owl:NamedIndividual .


###  http://purl.org/coreo#SituationType
coreo:SituationType rdf:type owl:NamedIndividual .


###  http://purl.org/coreo#Skill
coreo:Skill rdf:type owl:NamedIndividual ,
                     gufo:SubKind .


###  http://purl.org/coreo#SkillType
coreo:SkillType rdf:type owl:NamedIndividual .


###  http://purl.org/coreo#SocialAgent
coreo:SocialAgent rdf:type owl:NamedIndividual ,
                           gufo:Category .


###  http://purl.org/coreo#SubstantialType
coreo:SubstantialType rdf:type owl:NamedIndividual .


###  http://purl.org/coreo#TaskInput
coreo:TaskInput rdf:type owl:NamedIndividual ,
                         gufo:RoleMixin .


###  http://purl.org/coreo#TaskOutput
coreo:TaskOutput rdf:type owl:NamedIndividual ,
                          gufo:Category .


###  http://purl.org/coreo#TaskType
coreo:TaskType rdf:type owl:NamedIndividual .


###  http://purl.org/coreo#Type
coreo:Type rdf:type owl:NamedIndividual .


#################################################################
#    Annotations
#################################################################

coreo:Agent rdfs:comment "Agents are objects that perceive events and perform actions based on their intentions"@en ;
            rdfs:label "Agent"@en .


coreo:Artifact rdfs:comment """Human-made object produced, used, or changed in task as a result of human capabilities

E.G., Web form code (produced by John)""" ;
               rdfs:label "Artifact"@en .


coreo:ArtifactType gufo:categorizes coreo:Artifact ;
                   rdfs:comment """A gufo:Type whose instances are coreo:Artifact. 

Instances of coreo:ArtifactType are subclasses of coreo:Artifact.

Examples include \"Web Form\", \"Class Diagram\", \"Painting\", a \"Sculpture\""""@en ;
                   rdfs:label "ArtifactType"@en .


coreo:Attitude rdfs:comment """Attitude is a tendency to act (or feel) in a given situation (Maze, 2011) inherent to an individual, based on assumptions, values, and beliefs (Maze, 2011). In general, definitions of attitude take into account the following characteristics: (i) mental state; (ii) values (beliefs, 
emotions); and (iii) predisposition to act or behave (ALTMANN, 2008).

E.g. John' accuracy, Paul' responsability, Mary' colaboration

ALTMANN, Tanya K. Attitude: a concept analysis. In: Nursing forum. Malden, USA: Blackwell Publishing Inc, 2008. p. 144-150.

MAZE, John R. The concept of attitude. In: Realism and Psychology. Brill, 2011. p. 183-230."""@en ;
               rdfs:label "Attitude"@en .


coreo:AttitudeType rdfs:comment """A gufo:Type whose instances are coreo:Attitude. 

Instances of coreo:AttitudeType are subclasses of coreo:Attitude.

Examples include the coreo:HumanAttitude \"Collaboration\""""@en ;
                   rdfs:label "AttitudeType"@en .


coreo:CapabilityContext rdfs:label "Capability Context"@en .


coreo:CapabilityManifestation rdfs:label "Capability Manifestation"@en .


coreo:CapabilityOutcome rdfs:label "Capability Outcome"@en .


coreo:CapabilityRequiringRole gufo:categorizes coreo:Person ;
                              rdfs:label "CapabilityRequiringRole"@en .


coreo:CompetenceContext rdfs:label "Competence Context"@en ,
                                   "CompetenceContext"@en .


coreo:CompetenceOutcome rdfs:label "CompetenceOutcome"@en .


coreo:CompetenceType gufo:categorizes coreo:PersonalCompetence ;
                     rdfs:comment """A gufo:Type whose instances are coreo:PersonalCompetence. 

Instances of coreo:CompetenceType are subclasses of coreo:PersonalCompetence.

Examples include the competence type of \"Software Development\""""@en ;
                     rdfs:label "CompetenceType"@en .


coreo:Evidence rdfs:comment """Any object (social or not) used to prove a human capability. 
E.G.  John's graduation certification in computer science,  Mary's project participation."""@en ;
               rdfs:label "Evidence"@en .


coreo:Field rdfs:comment "Knowledge Area"@en ;
            rdfs:label "Field"@en .


coreo:HumanAspect rdfs:comment "Aspects inherent to an individual. Includes human capabilities (skills and competences), knowledge, attidutes, and other characteristics (human qualities as age, gender, etc and human traits)."@en ;
                  rdfs:label "HumanAspect"@en .


coreo:HumanAspectPhase gufo:categorizes coreo:HumanAspect ;
                       rdfs:label "HumanAspectPhase"@en .


coreo:HumanAspectType gufo:categorizes coreo:HumanAspect ;
                      rdfs:comment """A gufo:Type whose instances are coreo:HumanAspect. 

Instances of coreo:HumanAspectType are subclasses of coreo:HumanAspect.

Examples include the coreo:SkillType \"Java Programming\", the coreo:CompetenceType \"Software Development\", the coreo:HumanAttitude \"Collaboration\", the coreo:HumanKnowledge \"Quantum Physics\", the coreo:HumanCharacteristic \"Age\", \"Gender\", and \"Interest\""""@en ;
                      rdfs:label "HumanAspectType"@en .


coreo:HumanCapability rdfs:comment "Human ability to perform some task in some situation, inherent to an individual. Includes skills and personal competences."@en ;
                      rdfs:label "HumanCapability"@en .


coreo:HumanCapabilityType gufo:categorizes coreo:HumanCapability ;
                          rdfs:comment """A gufo:Type whose instances are dispositions. 

Instances of coreo:HumanCapabilityType are subclasses of coreo:HumanCapability.

Examples include the skill type of \"Java Programming\" and competence type of \"Software Development\""""@en ;
                          rdfs:label "HumanCapabilityType"@en .


coreo:HumanCharacteristic rdfs:comment "Human aspects inherent to an individual used to describe his/her profile, Includes qualities and traits"@en ;
                          rdfs:label "HumanCharacteristic"@en .


coreo:HumanQuality rdfs:comment "Qualities inherent to a person, e.g. age, gender, height, etc."@en ;
                   rdfs:label "HumanQuality"@en .


coreo:HumanTask rdfs:comment "Event performed by a person as a result of the manifestation of his/her human capabilities"@en ;
                rdfs:label "HumanTask"@en .


coreo:HumanTrait rdfs:comment "Traits inherent to an individual, e.g. John's introversion, Paul's interest, Mary's hobbies"@en ;
                 rdfs:label "HumanTrait"@en .


coreo:Knowledge rdfs:comment """Knowledge is typically associated with internal representations of facts, principles, or theories (WESTERA, 2001) by an individual. and that can be manifested through actions.

E.G., Paul' quantum theory knowledge

WESTERA, Wim. Competences in education: a confusion of tongues. Journal of Curriculum studies, v. 33, n. 1, p. 75-88, 2001."""@en ;
                rdfs:label "Knowledge"@en .


coreo:KnowledgeType rdfs:comment """A gufo:Type whose instances are coreo:Knowledge. 

Instances of coreo:KnowledgeType are subclasses of coreo:Knowledge.

Examples include the the coreo:KnowledgeType \"Quantum Physics\""""@en ;
                    rdfs:label "KnowledgeType"@en .


coreo:MomentType rdfs:comment """A gufo:Type whose instances are aspects. 

Instances of AspectType are subclasses of gufo:Aspect.

Examples include the aspect kind \"age\", \"knowledge\", and \"mariage\""""@en ;
                 rdfs:label "AspectType"@en .


coreo:Object rdfs:label "Object"@en .


coreo:Person rdfs:comment "Physical agent that are human being"@en ;
             rdfs:label "Person"@en .


coreo:PersonalCompetence rdfs:comment """Competence is a human capability inherent to an individual and formed by the combination of perceptible characteristics, such as the ``well-known'' knowledge, skills, and attitudes (KSA) elements. 


E.G. John's agile software development competence, Ronaldo's football playing competence"""@en ;
                         rdfs:label "PersonalCompetence"@en .


coreo:PersonalCompetenceType gufo:categorizes coreo:PersonalCompetence ;
                             rdfs:label "PersonalCompetenceType"@en .


coreo:Proficiency rdfs:comment "Intencity or deepness of a human capability. Can be related to level, degree, score, or other quality."@en ;
                  rdfs:label "Proficiency"@en .


coreo:Resource rdfs:comment """Any object used in a task by a person as manifestation of a human capability

E.G. John's Integrated Development Environment (IDE)"""@en ;
               rdfs:label "Resource"@en .


coreo:ResourceType gufo:categorizes coreo:Resource ;
                   rdfs:comment """A gufo:Type whose instances are coreo:Resource. 

Instances of coreo:ResourceType are subclasses of coreo:Resource.

Examples include \"Tool\", \"Software\", \"Hardware\""""@en ;
                   rdfs:label "ResourceType"@en .


coreo:Skill rdfs:comment """Skill is a human capability of an individual to perform a task (discrete unit of work) well (RODRIGUES et al, 2021), not strongly related to a context. 

E.G. John' programming skill, Pelé's kick skill


RODRIGUES, Margarida; FERNÁNDEZ-MACÍAS, Enrique; SOSTERO, Matteo. A unified conceptual framework of tasks, skills and competences. JRC Working Papers Series on Labour, Education and Technology, 2021."""@en ;
            rdfs:label "Skill"@en .


coreo:SkillType gufo:categorizes coreo:Skill ;
                rdfs:comment """A gufo:Type whose instances are coreo:Skill. 

Instances of coreo:SkillType are subclasses of coreo:Skill.

Examples include the skill type of \"Java Programming\""""@en ;
                rdfs:label "SkillType"@en .


coreo:SubstantialType rdfs:comment """A gufo:Type whose instances are objects. 

Instances of ObjectType are subclasses of Object.

Examples include the object kinds \"Car\", \"Person\", \"Apple\""""@en ;
                      rdfs:label "ObjectType"@en ,
                                 "SubstantialType"@en .


coreo:TaskInput rdfs:comment "Artifact used in a task as manifestation of a human capability"@en ;
                rdfs:label "TaskInput"@en .


coreo:TaskOutcome rdfs:label "Task Outcome"@en .


coreo:TaskOutput rdfs:comment "Artifact created or changed in a task as manifestation of a human capability"@en ;
                 rdfs:label "TaskOutput"@en .


coreo:TaskType gufo:categorizes coreo:HumanTask ;
               rdfs:comment """A gufo:Type whose instances are coreo:Task. 

Instances of coreo:TaskType are subclasses of coreo:Task.

Examples include \"Develop a Software\", \"Perform a Interview\""""@en ;
               rdfs:label "TaskType"@en .


#################################################################
#    General axioms
#################################################################

[ rdf:type owl:AllDisjointClasses ;
  owl:members ( coreo:Attitude
                coreo:HumanCapability
                coreo:HumanQuality
                coreo:HumanTrait
                coreo:Knowledge
              )
] .


[ rdf:type owl:AllDisjointClasses ;
  owl:members ( coreo:AttitudeType
                coreo:HumanCapabilityType
                coreo:KnowledgeType
              )
] .


###  Generated by the OWL API (version 4.5.25.2023-02-15T19:15:49Z) https://github.com/owlcs/owlapi
