@prefix : <http://purl.org/coreo#> .
@prefix owl: <http://www.w3.org/2002/07/owl#> .
@prefix rdf: <http://www.w3.org/1999/02/22-rdf-syntax-ns#> .
@prefix xml: <http://www.w3.org/XML/1998/namespace> .
@prefix xsd: <http://www.w3.org/2001/XMLSchema#> .
@prefix gufo: <http://purl.org/nemo/gufo#> .
@prefix rdfs: <http://www.w3.org/2000/01/rdf-schema#> .
@base <http://purl.org/coreo> .

<http://purl.org/coreo> rdf:type owl:Ontology ;
                         owl:versionIRI <http://purl.org/coreo/1.0.0> ;
                         owl:imports <http://purl.org/nemo/gufo#/1.0.0> ;
                         <http://purl.org/dc/elements/1.1/creator> """<https://orcid.org/0009-0006-6051-2165>,
<https://orcid.org/0000-0002-9819-3781>,
<https://orcid.org/0000-0002-5385-5761>,
<https://orcid.org/0000-0002-3452-553X>"""@en ;
                         <http://purl.org/dc/elements/1.1/title> "Core-o: Competence Reference Ontology"@en ;
                         <http://purl.org/dc/terms/bibliographicCitation> "R. F. Calhau, J. P. A. Almeida, T. P. Sales, G. Guizzardi, \\\"Core-O: A Competence Reference Ontology\\\", 2023, http://purl.org/coreo"@en ;
                         <http://purl.org/dc/terms/created> "2023-05-08"^^xsd:date ;
                         <http://purl.org/dc/terms/description> "An ontology to describe competences and human capabilities"@en ;
                         <http://purl.org/dc/terms/issued> "2023-05-08"^^xsd:date ;
                         <http://purl.org/dc/terms/license> "https://creativecommons.org/licenses/by/4.0/legalcode"^^xsd:anyURI ;
                         <http://purl.org/dc/terms/modified> "2023-05-12"^^xsd:date ;
                         <http://purl.org/dc/terms/publisher> "<https://www.utwente.nl/eemcs/scs/>"@en ;
                         <http://purl.org/vocab/vann/preferredNamespacePrefix> "coreo"@en ;
                         <http://purl.org/vocab/vann/preferredNamespaceUri> "http://purl.org/coreo"@en ;
                         rdfs:comment """Core-O is a well-founded competence reference ontology that accounts for competence-related elements such as knowledge, attitudes, and skills; also countenance their performance---related to tasks, their context, and outcomes---as well as their evolution over time (proficiency). This ontology is based on the Unified Foundational Ontology (Guizzardi, 2005), more specifically using gUFO (gentle UFO), a UFO-based lightweight ontology.
The ontology was based on these works: (CALHAU et al., 2021) and (CALHAU et al., 2023)

It was created to support: (i) semantically annotate competence-related artifacts such as curriculum, job vacancy, learning objects, resources, professional profiles, task logs, logbooks, and learning diaries; (ii) semantically inter-operate and integrate professional data concerning internal system (from organizations, VET institutions) and external ones (e.g., professional networks as LinkedIn); (iii) support the semantic search to find the best professional to an occupation, or to find the best occupation to a professional; (iv) support the skill/competence matching in gap analysis; (v) support competence/skill identification/assessment based on ontology-driven data and text mining in competence-related artifacts, such as learning diary, logbook, or task logs from control version tools as Github.


For background information on the reference ontology, see: 

1. CALHAU, Rodrigo F.; AZEVEDO, Carlos LB; ALMEIDA, João Paulo A. Towards Ontology-based Competence Modeling in Enterprise Architecture. In: 2021 IEEE 25th International Enterprise Distributed Object Computing Conference (EDOC). IEEE, 2021. p. 71-81.
2. CALHAU, Rodrigo F.; ALMEIDA, João Paulo A. Zooming in on Competences in Ontology-Based Enterprise Architecture Modeling. In: Enterprise Design, Operations, and Computing. EDOC 2022 Workshops: IDAMS, SoEA4EE, TEAR, EDOC Forum, Demonstrations Track and Doctoral Consortium, Bozen-Bolzano, Italy, October 4–7, 2022, Revised Selected Papers. Cham: Springer International Publishing, 2023. p. 198-213.
3. GUIZZARDI, Giancarlo. Ontological foundations for structural conceptual models. 2005.

Cite this work as: 
R. F. Calhau, J. P. A. Almeida, T. P. Sales, G. Guizzardi, \\\"Core-O: A Competence Reference Ontology\\\", 2023, http://purl.org/coreo

This work is distributed under Creative Commons Attribution License CC BY 4.0 <https://creativecommons.org/licenses/by/4.0/legalcode>.


For the source repository, see: <https://github.com/core-o/ontology>"""@en ;
                         owl:versionInfo "1.0.0"@en ;
                         <https://www.w3.org/1999/02/22-rdf-syntax-ns#type> "http://purl.org/vocommons/voaf#Vocabulary"@en .

#################################################################
#    Annotation properties
#################################################################

###  http://purl.org/dc/terms/description
<http://purl.org/dc/terms/description> rdf:type owl:AnnotationProperty .


###  http://purl.org/dc/terms/issued
<http://purl.org/dc/terms/issued> rdf:type owl:AnnotationProperty .


###  http://purl.org/dc/terms/publisher
<http://purl.org/dc/terms/publisher> rdf:type owl:AnnotationProperty .


###  http://purl.org/nemo/gufo#categorizes
gufo:categorizes rdf:type owl:AnnotationProperty .


###  http://purl.org/vocab/vann/preferredNamespacePrefix
<http://purl.org/vocab/vann/preferredNamespacePrefix> rdf:type owl:AnnotationProperty .


###  https://www.w3.org/1999/02/22-rdf-syntax-ns#type
<https://www.w3.org/1999/02/22-rdf-syntax-ns#type> rdf:type owl:AnnotationProperty .


#################################################################
#    Object Properties
#################################################################

###  http://purl.org/coreo#bringsAbout
:bringsAbout rdf:type owl:ObjectProperty ;
             rdfs:domain :TaskType ;
             rdfs:range gufo:SituationType ;
             rdfs:comment "Details the SituationType that a coreo:TaskType can result"@en ;
             rdfs:label "bringsAbout"@en .


###  http://purl.org/coreo#broughtAboutHumanTask
:broughtAboutHumanTask rdf:type owl:ObjectProperty ;
                       rdfs:subPropertyOf gufo:broughtAbout ;
                       rdfs:domain :CompetenceOutcome ;
                       rdfs:range :HumanTask ;
                       rdfs:label ""@en .


###  http://purl.org/coreo#capabilityRequiringRoleHasField
:capabilityRequiringRoleHasField rdf:type owl:ObjectProperty ;
                                 rdfs:domain :CapabilityRequiringRole ;
                                 rdfs:range :Field ;
                                 rdfs:comment "Describes the field of a coreo:CapabilityRequiringRole"@en ;
                                 rdfs:label "hasField"@en .


###  http://purl.org/coreo#characterizedBy
:characterizedBy rdf:type owl:ObjectProperty ;
                 rdfs:subPropertyOf :describedBy ;
                 rdfs:domain :ArtifactType ;
                 rdfs:range :MomentType ;
                 rdfs:comment "Relationship used to detail a coreo:ArtifactType"@en ;
                 rdfs:label "characterizedBy"@en .


###  http://purl.org/coreo#competenceContextContributedToTriggerHumanTask
:competenceContextContributedToTriggerHumanTask rdf:type owl:ObjectProperty ;
                                                rdfs:subPropertyOf gufo:contributedToTrigger ;
                                                rdfs:domain :CompetenceContext ;
                                                rdfs:range :HumanTask ;
                                                rdfs:comment "Identifies a coreo:HumanTask that the coreo:CompetenceContext contributed to trigger."@en ;
                                                rdfs:label "activatesTask"@en .


###  http://purl.org/coreo#concerns
:concerns rdf:type owl:ObjectProperty ;
          rdfs:subPropertyOf :describedBy ;
          rdfs:domain :TaskType ;
          rdfs:range :ArtifactType ;
          rdfs:comment "Relationship used to detail a coreo:TaskType"@en ;
          rdfs:label "concernsArtifact"@en .


###  http://purl.org/coreo#concerns_1
:concerns_1 rdf:type owl:ObjectProperty ;
            rdfs:subPropertyOf :describedBy ;
            rdfs:domain :TaskType ;
            rdfs:range :ResourceType ;
            rdfs:comment "Relationship used to detail a coreo:TaskType"@en ;
            rdfs:label "concernsResource"@en .


###  http://purl.org/coreo#constitutes
:constitutes rdf:type owl:ObjectProperty ;
             rdfs:subPropertyOf :constitutesType ;
             rdfs:domain :HumanAspectType ;
             rdfs:range :HumanAspectType ;
             rdfs:comment "Describes the constitutive relationship between coreo:HumanAspectTypes manifested as parthood relationships between their instances"@en ;
             rdfs:label "constitutesAspect"@en .


###  http://purl.org/coreo#constitutesType
:constitutesType rdf:type owl:ObjectProperty ;
                 rdfs:domain gufo:Type ;
                 rdfs:range gufo:Type ;
                 rdfs:comment "Describes the constitutive relationship between types manifested as parthood relationships between their instances"@en ;
                 rdfs:label "constitutesType"@en .


###  http://purl.org/coreo#contributesTo
:contributesTo rdf:type owl:ObjectProperty ;
               rdfs:domain :HumanQuality ;
               rdfs:range :PersonalCompetence ;
               rdfs:comment "Describes the contribution relation between a coreo:HumanQuality and a coreo:PersonalCompetence"@en ;
               rdfs:label "contributesTo"@en .


###  http://purl.org/coreo#definedInTermsOf
:definedInTermsOf rdf:type owl:ObjectProperty ;
                  rdfs:subPropertyOf :describedBy ;
                  rdfs:domain :HumanCapabilityType ;
                  rdfs:range :TaskType ;
                  rdfs:comment "Relationship used to detail a coreo:HumanCapabilityType"@en ;
                  rdfs:label "definedInTermsOf"@en .


###  http://purl.org/coreo#dependsOn
:dependsOn rdf:type owl:ObjectProperty ;
           rdfs:subPropertyOf :dependsOnType ;
           rdfs:domain :TaskType ;
           rdfs:range :TaskType ;
           rdfs:comment "Describes the dependence relationship between types manifested as dependence relationships between their instances"@en ;
           rdfs:label "dependsOnTask"@en .


###  http://purl.org/coreo#dependsOnType
:dependsOnType rdf:type owl:ObjectProperty ;
               rdfs:domain gufo:Type ;
               rdfs:range gufo:Type ;
               rdfs:comment "Describes the dependence relationship between types manifested as dependence relationships between their instances"@en ;
               rdfs:label "dependsOnType"@en .


###  http://purl.org/coreo#dependsOn_1
:dependsOn_1 rdf:type owl:ObjectProperty ;
             rdfs:subPropertyOf :dependsOnType ;
             rdfs:domain :ArtifactType ;
             rdfs:range :ArtifactType ;
             rdfs:comment "Describes the dependence relationship between types manifested as dependence relationships between their instances"@en ;
             rdfs:label "dependsOnArtifact"@en .


###  http://purl.org/coreo#dependsOn_2
:dependsOn_2 rdf:type owl:ObjectProperty ;
             rdfs:subPropertyOf :dependsOnType ;
             rdfs:domain :HumanAspectType ;
             rdfs:range :HumanAspectType ;
             rdfs:comment "Describes the dependence relationship between types manifested as dependence relationships between their instances"@en ;
             rdfs:label "dependsOnHumanAspect"@en .


###  http://purl.org/coreo#dependsOn_3
:dependsOn_3 rdf:type owl:ObjectProperty ;
             rdfs:subPropertyOf :dependsOnType ;
             rdfs:domain :CapabilityRequiringRole ;
             rdfs:range :CapabilityRequiringRole ;
             rdfs:comment "Describes the dependence relationship between types manifested as dependence relationships between their instances"@en ;
             rdfs:label "dependsOnRole"@en .


###  http://purl.org/coreo#describedBy
:describedBy rdf:type owl:ObjectProperty ;
             rdfs:domain gufo:Type ;
             rdfs:range gufo:Type ;
             rdfs:comment "Relationship used to detail a type"@en ;
             rdfs:label "describedBy"@en .


###  http://purl.org/coreo#enables
:enables rdf:type owl:ObjectProperty ;
         rdfs:domain :HumanCapabilityType ;
         rdfs:range gufo:SituationType ;
         rdfs:comment "Relationship used to detail types of contexts that activates HumanCapabilityTypes"@en ;
         rdfs:label "enablesSituationType"@en .


###  http://purl.org/coreo#evidencedBy
:evidencedBy rdf:type owl:ObjectProperty ;
             rdfs:domain :HumanAspect ;
             rdfs:range :Evidence ;
             rdfs:comment "evidances of a coreo:HumanAspect"@en ;
             rdfs:label "evidencedBy"@en .


###  http://purl.org/coreo#inheresIn
:inheresIn rdf:type owl:ObjectProperty ;
           rdfs:subPropertyOf gufo:inheresIn ;
           rdf:type owl:FunctionalProperty ,
                    owl:AsymmetricProperty ,
                    owl:IrreflexiveProperty ;
           rdfs:domain :Proficiency ;
           rdfs:range :HumanCapability ;
           rdfs:comment "relates a coreo:Proficiency to the correspondent coreo:HumanCapability"@en ;
           rdfs:label "inheresInHumanCapability"@en .


###  http://purl.org/coreo#inheresIn_1
:inheresIn_1 rdf:type owl:ObjectProperty ;
             rdfs:subPropertyOf :inheresIn_2 ;
             rdf:type owl:FunctionalProperty ,
                      owl:AsymmetricProperty ,
                      owl:IrreflexiveProperty ;
             rdfs:domain :HumanCapability ;
             rdfs:range :Person ;
             rdfs:comment "relates the coreo:HumanCapability to the correspondent coreo:Person"@en ;
             rdfs:label "CapabilityInheresInPerson"@en .


###  http://purl.org/coreo#inheresIn_2
:inheresIn_2 rdf:type owl:ObjectProperty ;
             rdfs:subPropertyOf gufo:inheresIn ;
             rdf:type owl:FunctionalProperty ,
                      owl:AsymmetricProperty ,
                      owl:IrreflexiveProperty ;
             rdfs:domain :HumanAspect ;
             rdfs:range :Person ;
             rdfs:comment "relates the coreo:HumanAspect to the correspondent coreo:Person"@en ;
             rdfs:label "inheresInPerson"@en .


###  http://purl.org/coreo#isDefinedBy
:isDefinedBy rdf:type owl:ObjectProperty ;
             rdfs:subPropertyOf :describedBy ;
             rdfs:domain :CapabilityRequiringRole ;
             rdfs:range :HumanCapabilityType ;
             rdfs:comment "Relationship used to detail a coreo:HumanCapabilityType"@en ;
             rdfs:label "isDefinedBy"@en .


###  http://purl.org/coreo#performed
:performed rdf:type owl:ObjectProperty ;
           rdfs:subPropertyOf gufo:participatedIn ;
           rdfs:domain :Person ;
           rdfs:range :HumanTask ;
           rdfs:comment "participation of a person in a human task"@en ;
           rdfs:label "performed"@en .


###  http://purl.org/coreo#personalCompetenceHasAttitude
:personalCompetenceHasAttitude rdf:type owl:ObjectProperty ;
                               rdfs:subPropertyOf gufo:isAspectProperPartOf ;
                               rdfs:domain :PersonalCompetence ;
                               rdfs:range :Attitude ;
                               rdfs:comment "parthood relation between a competence and attitude"@en ;
                               rdfs:label "hasAttitude"@en .


###  http://purl.org/coreo#personalCompetenceHasHumanAspect
:personalCompetenceHasHumanAspect rdf:type owl:ObjectProperty ;
                                  rdfs:subPropertyOf gufo:isAspectProperPartOf ;
                                  rdfs:domain :PersonalCompetence ;
                                  rdfs:range :HumanAspect ;
                                  rdfs:comment "parthood relation between a competence and human aspect"@en ;
                                  rdfs:label "hasHumanAspect"@en .


###  http://purl.org/coreo#personalCompetenceHasKnowledge
:personalCompetenceHasKnowledge rdf:type owl:ObjectProperty ;
                                rdfs:subPropertyOf gufo:isAspectProperPartOf ;
                                rdfs:domain :PersonalCompetence ;
                                rdfs:range :Knowledge ;
                                rdfs:comment "parthood relation between a competence and knowledge"@en ;
                                rdfs:label "hasKnowledge"@en .


###  http://purl.org/coreo#personalCompetenceHasPersonalCompetence
:personalCompetenceHasPersonalCompetence rdf:type owl:ObjectProperty ;
                                         rdfs:subPropertyOf gufo:isAspectProperPartOf ;
                                         rdfs:domain :PersonalCompetence ;
                                         rdfs:range :PersonalCompetence ;
                                         rdfs:comment "parthood relation between a competence and other competence"@en ;
                                         rdfs:label "hasCompetence"@en .


###  http://purl.org/coreo#personalCompetenceHasSkill
:personalCompetenceHasSkill rdf:type owl:ObjectProperty ;
                            rdfs:subPropertyOf gufo:isAspectProperPartOf ;
                            rdfs:domain :PersonalCompetence ;
                            rdfs:range :Skill ;
                            rdfs:comment "parthood relation between a competence and skill"@en ;
                            rdfs:label "hasSkill"@en .


###  http://purl.org/coreo#specializes
:specializes rdf:type owl:ObjectProperty ;
             rdfs:subPropertyOf :specializes_1 ;
             rdfs:domain :ArtifactType ;
             rdfs:range :ArtifactType ;
             rdfs:comment "specialization relation between types symbolizing the types that are instances of other type"@en ;
             rdfs:label "specializesArtifact"@en .


###  http://purl.org/coreo#specializes_1
:specializes_1 rdf:type owl:ObjectProperty ;
               rdfs:domain gufo:Type ;
               rdfs:range gufo:Type ;
               rdfs:comment "specialization relation between types symbolizing the types that are instances of other type"@en ;
               rdfs:label "specializes"@en .


###  http://purl.org/coreo#specializes_2
:specializes_2 rdf:type owl:ObjectProperty ;
               rdfs:subPropertyOf :specializes_1 ;
               rdfs:domain :HumanAspectType ;
               rdfs:range :HumanAspectType ;
               rdfs:comment "specialization relation between types symbolizing the types that are instances of other type"@en ;
               rdfs:label "specializesAspect"@en .


###  http://purl.org/coreo#specializes_3
:specializes_3 rdf:type owl:ObjectProperty ;
               rdfs:subPropertyOf :specializes_1 ;
               rdfs:domain :TaskType ;
               rdfs:range :TaskType ;
               rdfs:comment "specialization relation between types symbolizing the types that are instances of other type"@en ;
               rdfs:label "specializesTask"@en .


###  http://purl.org/coreo#specializes_4
:specializes_4 rdf:type owl:ObjectProperty ;
               rdfs:subPropertyOf :specializes_1 ;
               rdfs:domain :CapabilityRequiringRole ;
               rdfs:range :CapabilityRequiringRole ;
               rdfs:comment "specialization relation between types symbolizing the types that are instances of other type"@en ;
               rdfs:label "specializesRole"@en .


###  http://purl.org/coreo#standsIn
:standsIn rdf:type owl:ObjectProperty ;
          rdfs:subPropertyOf gufo:standsIn ;
          rdfs:domain :Resource ;
          rdfs:range :CompetenceContext ;
          rdfs:comment "Details the coreo:Resource that stands in a coreo:CompetenceContext"@en ;
          rdfs:label "standsInContext"@en .


###  http://purl.org/coreo#standsIn_1
:standsIn_1 rdf:type owl:ObjectProperty ;
            rdfs:subPropertyOf gufo:standsIn ;
            rdfs:domain :Artifact ;
            rdfs:range :CompetenceContext ;
            rdfs:comment "Details the coreo:Artifact that stands in a coreo:CompetenceContext"@en ;
            rdfs:label "standsInContext"@en .


###  http://purl.org/coreo#standsIn_2
:standsIn_2 rdf:type owl:ObjectProperty ;
            rdfs:subPropertyOf gufo:standsIn ;
            rdfs:domain :Artifact ;
            rdfs:range :CompetenceOutcome ;
            rdfs:comment "Details the coreo:Artifact that stands in a coreo:CompetenceOutcome"@en ;
            rdfs:label "standsInOutcome"@en .


###  http://purl.org/coreo#wasGeneratedIn
:wasGeneratedIn rdf:type owl:ObjectProperty ;
                rdfs:subPropertyOf gufo:wasCreatedIn ;
                rdfs:domain :TaskOutput ;
                rdfs:range :HumanTask ;
                rdfs:comment "output generation from a coreo:HumanTask"@en ;
                rdfs:label "wasGeneratedIn"@en .


###  http://purl.org/coreo#wasManifestedIn
:wasManifestedIn rdf:type owl:ObjectProperty ;
                 rdfs:subPropertyOf gufo:manifestedIn ;
                 rdfs:domain :HumanAspect ;
                 rdfs:range :HumanTask ;
                 rdfs:comment "Identifies a coreo:HumanTask in which the coreo:HumanAspect is manifested."@en ;
                 rdfs:label "wasManifestedInTask"@en .


###  http://purl.org/coreo#wasManifestedIn_1
:wasManifestedIn_1 rdf:type owl:ObjectProperty ;
                   rdfs:subPropertyOf gufo:manifestedIn ;
                   rdfs:domain :HumanCapability ;
                   rdfs:range :HumanTask ;
                   rdfs:comment "Identifies a coreo:HumanTask in which the coreo:HumanCapability is manifested."@en ;
                   rdfs:label "wasManifestedIn"@en .


###  http://purl.org/coreo#wasUsedIn
:wasUsedIn rdf:type owl:ObjectProperty ;
           rdfs:subPropertyOf gufo:participatedIn ;
           rdfs:domain :TaskInput ;
           rdfs:range :HumanTask ;
           rdfs:comment "usage of a artifact in a human task as input"@en ;
           rdfs:label "wasUsedIn"@en .


###  http://purl.org/coreo#wasUsedIn_1
:wasUsedIn_1 rdf:type owl:ObjectProperty ;
             rdfs:subPropertyOf gufo:participatedIn ;
             rdfs:domain :Resource ;
             rdfs:range :HumanTask ;
             rdfs:comment "usage of an object in a human task as a resource"@en ;
             rdfs:label "wasUsedIn"@en .


#################################################################
#    Classes
#################################################################

###  http://purl.org/coreo#Agent
:Agent rdf:type owl:Class ;
       rdfs:subClassOf gufo:Object .


###  http://purl.org/coreo#Artifact
:Artifact rdf:type owl:Class ;
          rdfs:subClassOf gufo:Object .


###  http://purl.org/coreo#ArtifactType
:ArtifactType rdf:type owl:Class ;
              rdfs:subClassOf :SubstantialType .


###  http://purl.org/coreo#Attitude
:Attitude rdf:type owl:Class ;
          rdfs:subClassOf :HumanAspect .


###  http://purl.org/coreo#AttitudeType
:AttitudeType rdf:type owl:Class ;
              rdfs:subClassOf :HumanAspectType .


###  http://purl.org/coreo#CapabilityRequiringRole
:CapabilityRequiringRole rdf:type owl:Class ;
                         rdfs:subClassOf gufo:Role .


###  http://purl.org/coreo#CompetenceContext
:CompetenceContext rdf:type owl:Class ;
                   rdfs:subClassOf gufo:Situation ,
                                   [ rdf:type owl:Restriction ;
                                     owl:onProperty :competenceContextContributedToTriggerHumanTask ;
                                     owl:someValuesFrom :HumanTask
                                   ] .


###  http://purl.org/coreo#CompetenceOutcome
:CompetenceOutcome rdf:type owl:Class ;
                   rdfs:subClassOf gufo:Situation .


###  http://purl.org/coreo#Evidence
:Evidence rdf:type owl:Class ;
          rdfs:subClassOf gufo:ConcreteIndividual .


###  http://purl.org/coreo#Field
:Field rdf:type owl:Class ;
       rdfs:subClassOf gufo:ConcreteIndividualType .


###  http://purl.org/coreo#HumanAspect
:HumanAspect rdf:type owl:Class ;
             rdfs:subClassOf gufo:IntrinsicMode ,
                             [ rdf:type owl:Restriction ;
                               owl:onProperty :inheresIn_2 ;
                               owl:qualifiedCardinality "1"^^xsd:nonNegativeInteger ;
                               owl:onClass :Person
                             ] .


###  http://purl.org/coreo#HumanAspectPhase
:HumanAspectPhase rdf:type owl:Class ;
                  rdfs:subClassOf :HumanAspectType ,
                                  gufo:Phase .


###  http://purl.org/coreo#HumanAspectType
:HumanAspectType rdf:type owl:Class ;
                 rdfs:subClassOf :MomentType .


###  http://purl.org/coreo#HumanCapability
:HumanCapability rdf:type owl:Class ;
                 owl:equivalentClass [ rdf:type owl:Class ;
                                       owl:unionOf ( :PersonalCompetence
                                                     :Skill
                                                   )
                                     ] ;
                 rdfs:subClassOf :HumanAspect ,
                                 [ rdf:type owl:Restriction ;
                                   owl:onProperty :wasManifestedIn_1 ;
                                   owl:someValuesFrom :HumanTask
                                 ] ,
                                 [ rdf:type owl:Restriction ;
                                   owl:onProperty [ owl:inverseOf :inheresIn
                                                  ] ;
                                   owl:someValuesFrom :Proficiency
                                 ] ,
                                 [ rdf:type owl:Restriction ;
                                   owl:onProperty :inheresIn_1 ;
                                   owl:qualifiedCardinality "1"^^xsd:nonNegativeInteger ;
                                   owl:onClass :Person
                                 ] .


###  http://purl.org/coreo#HumanCapabilityType
:HumanCapabilityType rdf:type owl:Class ;
                     rdfs:subClassOf :HumanAspectType .


###  http://purl.org/coreo#HumanQuality
:HumanQuality rdf:type owl:Class ;
              rdfs:subClassOf :HumanAspect .


###  http://purl.org/coreo#HumanTask
:HumanTask rdf:type owl:Class ;
           rdfs:subClassOf gufo:Event ,
                           [ rdf:type owl:Restriction ;
                             owl:onProperty [ owl:inverseOf :performed
                                            ] ;
                             owl:someValuesFrom :Person
                           ] ,
                           [ rdf:type owl:Restriction ;
                             owl:onProperty [ owl:inverseOf :wasGeneratedIn
                                            ] ;
                             owl:someValuesFrom :TaskOutput
                           ] ,
                           [ rdf:type owl:Restriction ;
                             owl:onProperty [ owl:inverseOf :wasManifestedIn
                                            ] ;
                             owl:someValuesFrom :HumanAspect
                           ] ,
                           [ rdf:type owl:Restriction ;
                             owl:onProperty [ owl:inverseOf :wasUsedIn
                                            ] ;
                             owl:someValuesFrom :TaskInput
                           ] ,
                           [ rdf:type owl:Restriction ;
                             owl:onProperty [ owl:inverseOf :wasUsedIn_1
                                            ] ;
                             owl:someValuesFrom :Resource
                           ] ,
                           [ rdf:type owl:Restriction ;
                             owl:onProperty [ owl:inverseOf :competenceContextContributedToTriggerHumanTask
                                            ] ;
                             owl:minQualifiedCardinality "1"^^xsd:nonNegativeInteger ;
                             owl:onClass :CompetenceContext
                           ] .


###  http://purl.org/coreo#HumanTrait
:HumanTrait rdf:type owl:Class ;
            rdfs:subClassOf :HumanAspect .


###  http://purl.org/coreo#Knowledge
:Knowledge rdf:type owl:Class ;
           rdfs:subClassOf :HumanAspect .


###  http://purl.org/coreo#KnowledgeType
:KnowledgeType rdf:type owl:Class ;
               rdfs:subClassOf :HumanAspectType .


###  http://purl.org/coreo#MomentType
:MomentType rdf:type owl:Class ;
            rdfs:subClassOf gufo:EndurantType .


###  http://purl.org/coreo#Object
:Object rdf:type owl:Class ;
        rdfs:subClassOf gufo:FunctionalComplex .


###  http://purl.org/coreo#Person
:Person rdf:type owl:Class ;
        rdfs:subClassOf :Agent ,
                        [ rdf:type owl:Restriction ;
                          owl:onProperty [ owl:inverseOf :inheresIn_1
                                         ] ;
                          owl:qualifiedCardinality "1"^^xsd:nonNegativeInteger ;
                          owl:onClass :HumanCapability
                        ] .


###  http://purl.org/coreo#PersonalCompetence
:PersonalCompetence rdf:type owl:Class ;
                    rdfs:subClassOf :HumanCapability ;
                    owl:disjointWith :Skill .


###  http://purl.org/coreo#PersonalCompetenceType
:PersonalCompetenceType rdf:type owl:Class ;
                        rdfs:subClassOf :HumanCapabilityType .


###  http://purl.org/coreo#Proficiency
:Proficiency rdf:type owl:Class ;
             rdfs:subClassOf gufo:Quality ,
                             [ rdf:type owl:Restriction ;
                               owl:onProperty :inheresIn ;
                               owl:qualifiedCardinality "1"^^xsd:nonNegativeInteger ;
                               owl:onClass :HumanCapability
                             ] .


###  http://purl.org/coreo#Resource
:Resource rdf:type owl:Class ;
          rdfs:subClassOf gufo:Object .


###  http://purl.org/coreo#ResourceType
:ResourceType rdf:type owl:Class ;
              rdfs:subClassOf :SubstantialType .


###  http://purl.org/coreo#Skill
:Skill rdf:type owl:Class ;
       rdfs:subClassOf :HumanCapability .


###  http://purl.org/coreo#SkillType
:SkillType rdf:type owl:Class ;
           rdfs:subClassOf :HumanCapabilityType .


###  http://purl.org/coreo#SubstantialType
:SubstantialType rdf:type owl:Class ;
                 rdfs:subClassOf gufo:EndurantType .


###  http://purl.org/coreo#TaskInput
:TaskInput rdf:type owl:Class ;
           rdfs:subClassOf :Artifact .


###  http://purl.org/coreo#TaskOutput
:TaskOutput rdf:type owl:Class ;
            rdfs:subClassOf :Artifact .


###  http://purl.org/coreo#TaskType
:TaskType rdf:type owl:Class ;
          rdfs:subClassOf gufo:EventType .


#################################################################
#    Individuals
#################################################################

###  http://purl.org/coreo#Agent
:Agent rdf:type owl:NamedIndividual ,
                gufo:Category .


###  http://purl.org/coreo#Artifact
:Artifact rdf:type owl:NamedIndividual ,
                   gufo:Category .


###  http://purl.org/coreo#ArtifactType
:ArtifactType rdf:type owl:NamedIndividual .


###  http://purl.org/coreo#Attitude
:Attitude rdf:type owl:NamedIndividual ,
                   gufo:Kind .


###  http://purl.org/coreo#AttitudeType
:AttitudeType rdf:type owl:NamedIndividual .


###  http://purl.org/coreo#CapabilityRequiringRole
:CapabilityRequiringRole rdf:type owl:NamedIndividual .


###  http://purl.org/coreo#CompetenceContext
:CompetenceContext rdf:type owl:NamedIndividual ,
                            gufo:SituationType .


###  http://purl.org/coreo#CompetenceOutcome
:CompetenceOutcome rdf:type owl:NamedIndividual ,
                            gufo:SituationType .


###  http://purl.org/coreo#EndurantType
:EndurantType rdf:type owl:NamedIndividual .


###  http://purl.org/coreo#Evidence
:Evidence rdf:type owl:NamedIndividual ,
                   gufo:Category .


###  http://purl.org/coreo#Field
:Field rdf:type owl:NamedIndividual .


###  http://purl.org/coreo#HumanAspect
:HumanAspect rdf:type owl:NamedIndividual ,
                      gufo:Category .


###  http://purl.org/coreo#HumanAspectPhase
:HumanAspectPhase rdf:type owl:NamedIndividual .


###  http://purl.org/coreo#HumanAspectType
:HumanAspectType rdf:type owl:NamedIndividual .


###  http://purl.org/coreo#HumanCapability
:HumanCapability rdf:type owl:NamedIndividual ,
                          gufo:Kind .


###  http://purl.org/coreo#HumanCapabilityType
:HumanCapabilityType rdf:type owl:NamedIndividual .


###  http://purl.org/coreo#HumanQuality
:HumanQuality rdf:type owl:NamedIndividual ,
                       gufo:Category .


###  http://purl.org/coreo#HumanTask
:HumanTask rdf:type owl:NamedIndividual ,
                    gufo:EventType .


###  http://purl.org/coreo#HumanTrait
:HumanTrait rdf:type owl:NamedIndividual ,
                     gufo:Category .


###  http://purl.org/coreo#Knowledge
:Knowledge rdf:type owl:NamedIndividual ,
                    gufo:Kind .


###  http://purl.org/coreo#KnowledgeType
:KnowledgeType rdf:type owl:NamedIndividual .


###  http://purl.org/coreo#MomentType
:MomentType rdf:type owl:NamedIndividual .


###  http://purl.org/coreo#Object
:Object rdf:type owl:NamedIndividual ,
                 gufo:Category .


###  http://purl.org/coreo#PerdurantType
:PerdurantType rdf:type owl:NamedIndividual .


###  http://purl.org/coreo#Person
:Person rdf:type owl:NamedIndividual ,
                 gufo:Kind .


###  http://purl.org/coreo#PersonalCompetence
:PersonalCompetence rdf:type owl:NamedIndividual ,
                             gufo:SubKind .


###  http://purl.org/coreo#PersonalCompetenceType
:PersonalCompetenceType rdf:type owl:NamedIndividual .


###  http://purl.org/coreo#Phase
:Phase rdf:type owl:NamedIndividual .


###  http://purl.org/coreo#PhysicalAgent
:PhysicalAgent rdf:type owl:NamedIndividual ,
                        gufo:Category .


###  http://purl.org/coreo#Proficiency
:Proficiency rdf:type owl:NamedIndividual ,
                      gufo:Kind .


###  http://purl.org/coreo#Resource
:Resource rdf:type owl:NamedIndividual ,
                   gufo:RoleMixin .


###  http://purl.org/coreo#ResourceType
:ResourceType rdf:type owl:NamedIndividual .


###  http://purl.org/coreo#Role
:Role rdf:type owl:NamedIndividual .


###  http://purl.org/coreo#SituationType
:SituationType rdf:type owl:NamedIndividual .


###  http://purl.org/coreo#Skill
:Skill rdf:type owl:NamedIndividual ,
                gufo:SubKind .


###  http://purl.org/coreo#SkillType
:SkillType rdf:type owl:NamedIndividual .


###  http://purl.org/coreo#SocialAgent
:SocialAgent rdf:type owl:NamedIndividual ,
                      gufo:Category .


###  http://purl.org/coreo#SubstantialType
:SubstantialType rdf:type owl:NamedIndividual .


###  http://purl.org/coreo#TaskInput
:TaskInput rdf:type owl:NamedIndividual ,
                    gufo:RoleMixin .


###  http://purl.org/coreo#TaskOutput
:TaskOutput rdf:type owl:NamedIndividual ,
                     gufo:Category .


###  http://purl.org/coreo#TaskType
:TaskType rdf:type owl:NamedIndividual .


###  http://purl.org/coreo#Type
:Type rdf:type owl:NamedIndividual .


#################################################################
#    Annotations
#################################################################

:Agent rdfs:label "Agent"@en ;
       rdfs:comment "Agents are objects that perceive events and perform actions based on their intentions"@en .


:Artifact rdfs:comment """Human-made object produced, used, or changed in task as a result of human capabilities

E.G., Web form code (produced by John)""" ;
          rdfs:label "Artifact"@en .


:ArtifactType rdfs:comment """A gufo:Type whose instances are coreo:Artifact. 

Instances of coreo:ArtifactType are subclasses of coreo:Artifact.

Examples include \"Web Form\", \"Class Diagram\", \"Painting\", a \"Sculpture\""""@en ;
              gufo:categorizes :Artifact ;
              rdfs:label "ArtifactType"@en .


:Attitude rdfs:comment """Attitude is a tendency to act (or feel) in a given situation (Maze, 2011) inherent to an individual, based on assumptions, values, and beliefs (Maze, 2011). In general, definitions of attitude take into account the following characteristics: (i) mental state; (ii) values (beliefs, 
emotions); and (iii) predisposition to act or behave (ALTMANN, 2008).

E.g. John' accuracy, Paul' responsability, Mary' colaboration

ALTMANN, Tanya K. Attitude: a concept analysis. In: Nursing forum. Malden, USA: Blackwell Publishing Inc, 2008. p. 144-150.

MAZE, John R. The concept of attitude. In: Realism and Psychology. Brill, 2011. p. 183-230."""@en ;
          rdfs:label "Attitude"@en .


:AttitudeType rdfs:label "AttitudeType"@en ;
              rdfs:comment """A gufo:Type whose instances are coreo:Attitude. 

Instances of coreo:AttitudeType are subclasses of coreo:Attitude.

Examples include the coreo:HumanAttitude \"Collaboration\""""@en .


:CapabilityContext rdfs:label "Capability Context"@en .


:CapabilityManifestation rdfs:label "Capability Manifestation"@en .


:CapabilityOutcome rdfs:label "Capability Outcome"@en .


:CapabilityRequiringRole rdfs:label "CapabilityRequiringRole"@en ;
                         gufo:categorizes :Person .


:CompetenceContext rdfs:label "CompetenceContext"@en ,
                              "Competence Context"@en .


:CompetenceOutcome rdfs:label "CompetenceOutcome"@en .


:CompetenceType gufo:categorizes :PersonalCompetence ;
                rdfs:label "CompetenceType"@en ;
                rdfs:comment """A gufo:Type whose instances are coreo:PersonalCompetence. 

Instances of coreo:CompetenceType are subclasses of coreo:PersonalCompetence.

Examples include the competence type of \"Software Development\""""@en .


:Evidence rdfs:label "Evidence"@en ;
          rdfs:comment """Any object (social or not) used to prove a human capability. 
E.G.  John's graduation certification in computer science,  Mary's project participation."""@en .


:Field rdfs:label "Field"@en ;
       rdfs:comment "Knowledge Area"@en .


:HumanAspect rdfs:comment "Aspects inherent to an individual. Includes human capabilities (skills and competences), knowledge, attidutes, and other characteristics (human qualities as age, gender, etc and human traits)."@en ;
             rdfs:label "HumanAspect"@en .


:HumanAspectPhase rdfs:label "HumanAspectPhase"@en ;
                  gufo:categorizes :HumanAspect .


:HumanAspectType gufo:categorizes :HumanAspect ;
                 rdfs:comment """A gufo:Type whose instances are coreo:HumanAspect. 

Instances of coreo:HumanAspectType are subclasses of coreo:HumanAspect.

Examples include the coreo:SkillType \"Java Programming\", the coreo:CompetenceType \"Software Development\", the coreo:HumanAttitude \"Collaboration\", the coreo:HumanKnowledge \"Quantum Physics\", the coreo:HumanCharacteristic \"Age\", \"Gender\", and \"Interest\""""@en ;
                 rdfs:label "HumanAspectType"@en .


:HumanCapability rdfs:label "HumanCapability"@en ;
                 rdfs:comment "Human ability to perform some task in some situation, inherent to an individual. Includes skills and personal competences."@en .


:HumanCapabilityType gufo:categorizes :HumanCapability ;
                     rdfs:comment """A gufo:Type whose instances are dispositions. 

Instances of coreo:HumanCapabilityType are subclasses of coreo:HumanCapability.

Examples include the skill type of \"Java Programming\" and competence type of \"Software Development\""""@en ;
                     rdfs:label "HumanCapabilityType"@en .


:HumanCharacteristic rdfs:label "HumanCharacteristic"@en ;
                     rdfs:comment "Human aspects inherent to an individual used to describe his/her profile, Includes qualities and traits"@en .


:HumanQuality rdfs:comment "Qualities inherent to a person, e.g. age, gender, height, etc."@en ;
              rdfs:label "HumanQuality"@en .


:HumanTask rdfs:comment "Event performed by a person as a result of the manifestation of his/her human capabilities"@en ;
           rdfs:label "HumanTask"@en .


:HumanTrait rdfs:comment "Traits inherent to an individual, e.g. John's introversion, Paul's interest, Mary's hobbies"@en ;
            rdfs:label "HumanTrait"@en .


:Knowledge rdfs:label "Knowledge"@en ;
           rdfs:comment """Knowledge is typically associated with internal representations of facts, principles, or theories (WESTERA, 2001) by an individual. and that can be manifested through actions.

E.G., Paul' quantum theory knowledge

WESTERA, Wim. Competences in education: a confusion of tongues. Journal of Curriculum studies, v. 33, n. 1, p. 75-88, 2001."""@en .


:KnowledgeType rdfs:comment """A gufo:Type whose instances are coreo:Knowledge. 

Instances of coreo:KnowledgeType are subclasses of coreo:Knowledge.

Examples include the the coreo:KnowledgeType \"Quantum Physics\""""@en ;
               rdfs:label "KnowledgeType"@en .


:MomentType rdfs:comment """A gufo:Type whose instances are aspects. 

Instances of AspectType are subclasses of gufo:Aspect.

Examples include the aspect kind \"age\", \"knowledge\", and \"mariage\""""@en ;
            rdfs:label "AspectType"@en .


:Object rdfs:label "Object"@en .


:Person rdfs:label "Person"@en ;
        rdfs:comment "Physical agent that are human being"@en .


:PersonalCompetence rdfs:comment """Competence is a human capability inherent to an individual and formed by the combination of perceptible characteristics, such as the ``well-known'' knowledge, skills, and attitudes (KSA) elements. 


E.G. John's agile software development competence, Ronaldo's football playing competence"""@en ;
                    rdfs:label "PersonalCompetence"@en .


:PersonalCompetenceType gufo:categorizes :PersonalCompetence ;
                        rdfs:label "PersonalCompetenceType"@en .


:Proficiency rdfs:label "Proficiency"@en ;
             rdfs:comment "Intencity or deepness of a human capability. Can be related to level, degree, score, or other quality."@en .


:Resource rdfs:label "Resource"@en ;
          rdfs:comment """Any object used in a task by a person as manifestation of a human capability

E.G. John's Integrated Development Environment (IDE)"""@en .


:ResourceType gufo:categorizes :Resource ;
              rdfs:comment """A gufo:Type whose instances are coreo:Resource. 

Instances of coreo:ResourceType are subclasses of coreo:Resource.

Examples include \"Tool\", \"Software\", \"Hardware\""""@en ;
              rdfs:label "ResourceType"@en .


:Skill rdfs:label "Skill"@en ;
       rdfs:comment """Skill is a human capability of an individual to perform a task (discrete unit of work) well (RODRIGUES et al, 2021), not strongly related to a context. 

E.G. John' programming skill, Pelé's kick skill


RODRIGUES, Margarida; FERNÁNDEZ-MACÍAS, Enrique; SOSTERO, Matteo. A unified conceptual framework of tasks, skills and competences. JRC Working Papers Series on Labour, Education and Technology, 2021."""@en .


:SkillType gufo:categorizes :Skill ;
           rdfs:comment """A gufo:Type whose instances are coreo:Skill. 

Instances of coreo:SkillType are subclasses of coreo:Skill.

Examples include the skill type of \"Java Programming\""""@en ;
           rdfs:label "SkillType"@en .


:SubstantialType rdfs:comment """A gufo:Type whose instances are objects. 

Instances of ObjectType are subclasses of Object.

Examples include the object kinds \"Car\", \"Person\", \"Apple\""""@en ;
                 rdfs:label "ObjectType"@en ,
                            "SubstantialType"@en .


:TaskInput rdfs:comment "Artifact used in a task as manifestation of a human capability"@en ;
           rdfs:label "TaskInput"@en .


:TaskOutcome rdfs:label "Task Outcome"@en .


:TaskOutput rdfs:label "TaskOutput"@en ;
            rdfs:comment "Artifact created or changed in a task as manifestation of a human capability"@en .


:TaskType rdfs:comment """A gufo:Type whose instances are coreo:Task. 

Instances of coreo:TaskType are subclasses of coreo:Task.

Examples include \"Develop a Software\", \"Perform a Interview\""""@en ;
          rdfs:label "TaskType"@en ;
          gufo:categorizes :HumanTask .


#################################################################
#    General axioms
#################################################################

[ rdf:type owl:AllDisjointClasses ;
  owl:members ( :Attitude
                :HumanCapability
                :HumanQuality
                :HumanTrait
                :Knowledge
              )
] .


[ rdf:type owl:AllDisjointClasses ;
  owl:members ( :AttitudeType
                :HumanCapabilityType
                :KnowledgeType
              )
] .


###  Generated by the OWL API (version 4.5.9.2019-02-01T07:24:44Z) https://github.com/owlcs/owlapi
